proof-libs/coq/ssprove/src/Hacspec_Lib_Integers.v
@@ -36,6 +36,8 @@ Open Scope list_scope.
 
 Import choice.Choice.Exports.
 
+From Hacspec Require Import Hacspec_Lib_StdLib.
+
 (* Definition lift3_both_ {A B C D : choice_type} {L} {I} (f : A -> B -> C -> D) (x : both L I A) (y : both L I B) (z : both L I C) := *)
 (*   bind_both_ x (fun x' => *)
 (*   bind_both_ y (fun y' => *)
@@ -43,172 +45,172 @@ Import choice.Choice.Exports.
 (*   ret_both (f x' y' z')))). *)
 
 Equations int_add {L1 L2 (* L3 *) : {fset Location}} {I1 I2 (* I3 *) : Interface} {WS}
-           (x : both L1 I1 (int WS)) (y : both L2 I2 (int WS))
-           (* `{H_loc_incl_x : is_true (fsubset L1 L3)} `{H_opsig_incl_x : is_true (fsubset I1 I3)} *)
-           (* `{H_loc_incl_y : is_true (fsubset L2 L3)} `{H_opsig_incl_y : is_true (fsubset I2 I3)} *) : both (L1 :|: L2) (* L3 *) (I1 :|: I2) (* I3 *) (int WS) :=
+  (x : both L1 I1 (int WS)) (y : both L2 I2 (int WS))
+  (* `{H_loc_incl_x : is_true (fsubset L1 L3)} `{H_opsig_incl_x : is_true (fsubset I1 I3)} *)
+  (* `{H_loc_incl_y : is_true (fsubset L2 L3)} `{H_opsig_incl_y : is_true (fsubset I2 I3)} *) : both (L1 :|: L2) (* L3 *) (I1 :|: I2) (* I3 *) (int WS) :=
   int_add := lift2_both (Hacspec_Lib_Pre.int_add).
-  Fail Next Obligation.
+Fail Next Obligation.
 
-  Equations int_sub {L1 L2 (* L3 *) : {fset Location}} {I1 I2 (* I3 *) : Interface} {WS}
-           (x : both L1 I1 (int WS)) (y : both L2 I2 (int WS))
-           (* `{H_loc_incl_x : is_true (fsubset L1 L3)} `{H_opsig_incl_x : is_true (fsubset I1 I3)} *)
-           (* `{H_loc_incl_y : is_true (fsubset L2 L3)} `{H_opsig_incl_y : is_true (fsubset I2 I3)} *) : both (L1 :|: L2) (* L3 *) (I1 :|: I2) (* I3 *) (int WS) :=
-    int_sub := (lift2_both (Hacspec_Lib_Pre.int_sub)).
-  Fail Next Obligation.
+Equations int_sub {L1 L2 (* L3 *) : {fset Location}} {I1 I2 (* I3 *) : Interface} {WS}
+  (x : both L1 I1 (int WS)) (y : both L2 I2 (int WS))
+  (* `{H_loc_incl_x : is_true (fsubset L1 L3)} `{H_opsig_incl_x : is_true (fsubset I1 I3)} *)
+  (* `{H_loc_incl_y : is_true (fsubset L2 L3)} `{H_opsig_incl_y : is_true (fsubset I2 I3)} *) : both (L1 :|: L2) (* L3 *) (I1 :|: I2) (* I3 *) (int WS) :=
+  int_sub := (lift2_both (Hacspec_Lib_Pre.int_sub)).
+Fail Next Obligation.
 
-  Equations int_opp {L (* L2 *) : {fset Location}} {I (* I2 *) : Interface} {WS}
-           (x : both L I (int WS))
-           (* `{H_loc_incl_x : is_true (fsubset L L2)} `{H_opsig_incl_x : is_true (fsubset I I2)} *) : both L I (int WS) :=
-    int_opp := (lift1_both (Hacspec_Lib_Pre.int_opp)).
-  Fail Next Obligation.
+Equations int_opp {L (* L2 *) : {fset Location}} {I (* I2 *) : Interface} {WS}
+  (x : both L I (int WS))
+  (* `{H_loc_incl_x : is_true (fsubset L L2)} `{H_opsig_incl_x : is_true (fsubset I I2)} *) : both L I (int WS) :=
+  int_opp := (lift1_both (Hacspec_Lib_Pre.int_opp)).
+Fail Next Obligation.
 
-  Equations int_mul {L1 L2 (* L3 *) : {fset Location}} {I1 I2 (* I3 *) : Interface} {WS}
-           (x : both L1 I1 (int WS)) (y : both L2 I2 (int WS))
-           (* `{H_loc_incl_x : is_true (fsubset L1 L3)} `{H_opsig_incl_x : is_true (fsubset I1 I3)} *)
-           (* `{H_loc_incl_y : is_true (fsubset L2 L3)} `{H_opsig_incl_y : is_true (fsubset I2 I3)} *) : both (L1 :|: L2) (* L3 *) (I1 :|: I2) (* I3 *) (int WS) :=
-    int_mul := (lift2_both (Hacspec_Lib_Pre.int_mul)).
-  Fail Next Obligation.
+Equations int_mul {L1 L2 (* L3 *) : {fset Location}} {I1 I2 (* I3 *) : Interface} {WS}
+  (x : both L1 I1 (int WS)) (y : both L2 I2 (int WS))
+  (* `{H_loc_incl_x : is_true (fsubset L1 L3)} `{H_opsig_incl_x : is_true (fsubset I1 I3)} *)
+  (* `{H_loc_incl_y : is_true (fsubset L2 L3)} `{H_opsig_incl_y : is_true (fsubset I2 I3)} *) : both (L1 :|: L2) (* L3 *) (I1 :|: I2) (* I3 *) (int WS) :=
+  int_mul := (lift2_both (Hacspec_Lib_Pre.int_mul)).
+Fail Next Obligation.
 
-  Equations int_div {L1 L2 (* L3 *) : {fset Location}} {I1 I2 (* I3 *) : Interface} {WS}
-           (x : both L1 I1 (int WS)) (y : both L2 I2 (int WS))
-           (* `{H_loc_incl_x : is_true (fsubset L1 L3)} `{H_opsig_incl_x : is_true (fsubset I1 I3)} *)
-           (* `{H_loc_incl_y : is_true (fsubset L2 L3)} `{H_opsig_incl_y : is_true (fsubset I2 I3)} *) : both (L1 :|: L2) (* L3 *) (I1 :|: I2) (* I3 *) (int WS) :=
-    int_div := (lift2_both (Hacspec_Lib_Pre.int_div : int _ -> int _ -> int _)).
-  Fail Next Obligation.
+Equations int_div {L1 L2 (* L3 *) : {fset Location}} {I1 I2 (* I3 *) : Interface} {WS}
+  (x : both L1 I1 (int WS)) (y : both L2 I2 (int WS))
+  (* `{H_loc_incl_x : is_true (fsubset L1 L3)} `{H_opsig_incl_x : is_true (fsubset I1 I3)} *)
+  (* `{H_loc_incl_y : is_true (fsubset L2 L3)} `{H_opsig_incl_y : is_true (fsubset I2 I3)} *) : both (L1 :|: L2) (* L3 *) (I1 :|: I2) (* I3 *) (int WS) :=
+  int_div := (lift2_both (Hacspec_Lib_Pre.int_div : int _ -> int _ -> int _)).
+Fail Next Obligation.
 
-  Equations int_mod {L1 L2 (* L3 *) : {fset Location}} {I1 I2 (* I3 *) : Interface} {WS}
-           (x : both L1 I1 (int WS)) (y : both L2 I2 (int WS))
-           (* `{H_loc_incl_x : is_true (fsubset L1 L3)} `{H_opsig_incl_x : is_true (fsubset I1 I3)} *)
-           (* `{H_loc_incl_y : is_true (fsubset L2 L3)} `{H_opsig_incl_y : is_true (fsubset I2 I3)} *) : both (L1 :|: L2) (* L3 *) (I1 :|: I2) (* I3 *) (int WS) :=
-    int_mod := (lift2_both (Hacspec_Lib_Pre.int_mod : int _ -> int _ -> int _)).
-  Fail Next Obligation.
+Equations int_mod {L1 L2 (* L3 *) : {fset Location}} {I1 I2 (* I3 *) : Interface} {WS}
+  (x : both L1 I1 (int WS)) (y : both L2 I2 (int WS))
+  (* `{H_loc_incl_x : is_true (fsubset L1 L3)} `{H_opsig_incl_x : is_true (fsubset I1 I3)} *)
+  (* `{H_loc_incl_y : is_true (fsubset L2 L3)} `{H_opsig_incl_y : is_true (fsubset I2 I3)} *) : both (L1 :|: L2) (* L3 *) (I1 :|: I2) (* I3 *) (int WS) :=
+  int_mod := (lift2_both (Hacspec_Lib_Pre.int_mod : int _ -> int _ -> int _)).
+Fail Next Obligation.
 
-  Equations int_xor {L1 L2 (* L3 *) : {fset Location}} {I1 I2 (* I3 *) : Interface} {WS}
-           (x : both L1 I1 (int WS)) (y : both L2 I2 (int WS))
-           (* `{H_loc_incl_x : is_true (fsubset L1 L3)} `{H_opsig_incl_x : is_true (fsubset I1 I3)} *)
-           (* `{H_loc_incl_y : is_true (fsubset L2 L3)} `{H_opsig_incl_y : is_true (fsubset I2 I3)} *) : both (L1 :|: L2) (* L3 *) (I1 :|: I2) (* I3 *) (int WS) :=
-    int_xor := (lift2_both (Hacspec_Lib_Pre.int_xor : int _ -> int _ -> int _)).
-  Fail Next Obligation.
+Equations int_xor {L1 L2 (* L3 *) : {fset Location}} {I1 I2 (* I3 *) : Interface} {WS}
+  (x : both L1 I1 (int WS)) (y : both L2 I2 (int WS))
+  (* `{H_loc_incl_x : is_true (fsubset L1 L3)} `{H_opsig_incl_x : is_true (fsubset I1 I3)} *)
+  (* `{H_loc_incl_y : is_true (fsubset L2 L3)} `{H_opsig_incl_y : is_true (fsubset I2 I3)} *) : both (L1 :|: L2) (* L3 *) (I1 :|: I2) (* I3 *) (int WS) :=
+  int_xor := (lift2_both (Hacspec_Lib_Pre.int_xor : int _ -> int _ -> int _)).
+Fail Next Obligation.
 
-  Equations int_and {L1 L2 (* L3 *) : {fset Location}} {I1 I2 (* I3 *) : Interface} {WS}
-           (x : both L1 I1 (int WS)) (y : both L2 I2 (int WS))
-           (* `{H_loc_incl_x : is_true (fsubset L1 L3)} `{H_opsig_incl_x : is_true (fsubset I1 I3)} *)
-           (* `{H_loc_incl_y : is_true (fsubset L2 L3)} `{H_opsig_incl_y : is_true (fsubset I2 I3)} *) : both (L1 :|: L2) (* L3 *) (I1 :|: I2) (* I3 *) (int WS) :=
-    int_and := (lift2_both (Hacspec_Lib_Pre.int_and : int _ -> int _ -> int _)).
-    Fail Next Obligation.
+Equations int_and {L1 L2 (* L3 *) : {fset Location}} {I1 I2 (* I3 *) : Interface} {WS}
+  (x : both L1 I1 (int WS)) (y : both L2 I2 (int WS))
+  (* `{H_loc_incl_x : is_true (fsubset L1 L3)} `{H_opsig_incl_x : is_true (fsubset I1 I3)} *)
+  (* `{H_loc_incl_y : is_true (fsubset L2 L3)} `{H_opsig_incl_y : is_true (fsubset I2 I3)} *) : both (L1 :|: L2) (* L3 *) (I1 :|: I2) (* I3 *) (int WS) :=
+  int_and := (lift2_both (Hacspec_Lib_Pre.int_and : int _ -> int _ -> int _)).
+Fail Next Obligation.
 
-    Equations int_or {L1 L2 (* L3 *) : {fset Location}} {I1 I2 (* I3 *) : Interface} {WS}
-           (x : both L1 I1 (int WS)) (y : both L2 I2 (int WS))
-           (* `{H_loc_incl_x : is_true (fsubset L1 L3)} `{H_opsig_incl_x : is_true (fsubset I1 I3)} *)
-           (* `{H_loc_incl_y : is_true (fsubset L2 L3)} `{H_opsig_incl_y : is_true (fsubset I2 I3)} *) : both (L1 :|: L2) (* L3 *) (I1 :|: I2) (* I3 *) (int WS) :=
-    int_or := (lift2_both (Hacspec_Lib_Pre.int_or : int _ -> int _ -> int _)).
-  Fail Next Obligation.
+Equations int_or {L1 L2 (* L3 *) : {fset Location}} {I1 I2 (* I3 *) : Interface} {WS}
+  (x : both L1 I1 (int WS)) (y : both L2 I2 (int WS))
+  (* `{H_loc_incl_x : is_true (fsubset L1 L3)} `{H_opsig_incl_x : is_true (fsubset I1 I3)} *)
+  (* `{H_loc_incl_y : is_true (fsubset L2 L3)} `{H_opsig_incl_y : is_true (fsubset I2 I3)} *) : both (L1 :|: L2) (* L3 *) (I1 :|: I2) (* I3 *) (int WS) :=
+  int_or := (lift2_both (Hacspec_Lib_Pre.int_or : int _ -> int _ -> int _)).
+Fail Next Obligation.
 
-  Equations int_not {L (* L2 *) : {fset Location}} {I (* I2 *) : Interface} {WS}
-           (x : both L I (int WS))
-           (* `{H_loc_incl_x : is_true (fsubset L1 L2)} `{H_opsig_incl_x : is_true (fsubset I1 I2)} *) : both L I (int WS) :=
-    int_not := (lift1_both (Hacspec_Lib_Pre.int_not : int _ -> int _)).
-  Fail Next Obligation.
+Equations int_not {L (* L2 *) : {fset Location}} {I (* I2 *) : Interface} {WS}
+  (x : both L I (int WS))
+  (* `{H_loc_incl_x : is_true (fsubset L1 L2)} `{H_opsig_incl_x : is_true (fsubset I1 I2)} *) : both L I (int WS) :=
+  int_not := (lift1_both (Hacspec_Lib_Pre.int_not : int _ -> int _)).
+Fail Next Obligation.
 
-  Equations cast_int {L (* L2 *) : {fset Location}} {I (* I2 *) : Interface} {WS1 WS2}
-           (x : both L I (int WS1))
-           (* `{H_loc_incl_x : is_true (fsubset L1 L2)} `{H_opsig_incl_x : is_true (fsubset I1 I2)} *) : both L I (int WS2) :=
-    cast_int := (lift1_both (fun (n : int _) => repr _ (unsigned n))).
-  Fail Next Obligation.
+Equations cast_int {L (* L2 *) : {fset Location}} {I (* I2 *) : Interface} {WS1 WS2}
+  (x : both L I (int WS1))
+  (* `{H_loc_incl_x : is_true (fsubset L1 L2)} `{H_opsig_incl_x : is_true (fsubset I1 I2)} *) : both L I (int WS2) :=
+  cast_int := (lift1_both (fun (n : int _) => repr _ (unsigned n))).
+Fail Next Obligation.
 (* End IntType. *)
 
 Notation secret := (lift1_both secret).
 
 Infix ".%%" := int_modi (at level 40, left associativity) : Z_scope.
-Infix ".+" := int_add (at level 77) : hacspec_scope.
-Infix ".-" := int_sub (at level 77) : hacspec_scope.
+(* Infix ".+" := int_add (at level 77) : hacspec_scope. *)
+(* Infix ".-" := int_sub (at level 77) : hacspec_scope. *)
 Notation "-" := int_opp (at level 77) : hacspec_scope.
-Infix ".*" := int_mul (at level 77) : hacspec_scope.
+(* Infix ".*" := int_mul (at level 77) : hacspec_scope. *)
 Infix "./" := int_div (at level 77) : hacspec_scope.
 Infix ".%" := int_mod (at level 77) : hacspec_scope.
-Infix ".^" := int_xor (at level 77) : hacspec_scope.
+(* Infix ".^" := int_xor (at level 77) : hacspec_scope. *)
 Infix ".&" := int_and (at level 77) : hacspec_scope.
 Infix ".|" := int_or (at level 77) : hacspec_scope.
 Notation "'not'" := int_not (at level 77) : hacspec_scope.
 
 (* Section Uint. *)
-  Notation uint8_declassify := (lift1_both uint8_declassify).
-  Notation int8_declassify := (lift1_both int8_declassify).
-  Notation uint16_declassify := (lift1_both uint16_declassify).
-  Notation int16_declassify := (lift1_both int16_declassify).
-  Notation uint32_declassify := (lift1_both uint32_declassify).
-  Notation int32_declassify := (lift1_both int32_declassify).
-  Notation uint64_declassify := (lift1_both uint64_declassify).
-  Notation int64_declassify := (lift1_both int64_declassify).
-  Notation uint128_declassify := (lift1_both uint128_declassify).
-  Notation int128_declassify := (lift1_both int128_declassify).
+Notation uint8_declassify := (lift1_both uint8_declassify).
+Notation int8_declassify := (lift1_both int8_declassify).
+Notation uint16_declassify := (lift1_both uint16_declassify).
+Notation int16_declassify := (lift1_both int16_declassify).
+Notation uint32_declassify := (lift1_both uint32_declassify).
+Notation int32_declassify := (lift1_both int32_declassify).
+Notation uint64_declassify := (lift1_both uint64_declassify).
+Notation int64_declassify := (lift1_both int64_declassify).
+Notation uint128_declassify := (lift1_both uint128_declassify).
+Notation int128_declassify := (lift1_both int128_declassify).
 
-  Notation uint8_classify := (lift1_both uint8_classify).
-  Notation int8_classify := (lift1_both int8_classify).
-  Notation uint16_classify := (lift1_both uint16_classify).
-  Notation int16_classify := (lift1_both int16_classify).
-  Notation uint32_classify := (lift1_both uint32_classify).
-  Notation int32_classify := (lift1_both int32_classify).
-  Notation uint64_classify := (lift1_both uint64_classify).
-  Notation int64_classify := (lift1_both int64_classify).
-  Notation uint128_classify := (lift1_both uint128_classify).
-  Notation int128_classify := (lift1_both int128_classify).
+Notation uint8_classify := (lift1_both uint8_classify).
+Notation int8_classify := (lift1_both int8_classify).
+Notation uint16_classify := (lift1_both uint16_classify).
+Notation int16_classify := (lift1_both int16_classify).
+Notation uint32_classify := (lift1_both uint32_classify).
+Notation int32_classify := (lift1_both int32_classify).
+Notation uint64_classify := (lift1_both uint64_classify).
+Notation int64_classify := (lift1_both int64_classify).
+Notation uint128_classify := (lift1_both uint128_classify).
+Notation int128_classify := (lift1_both int128_classify).
 
-  (* CompCert integers' signedness is only interpreted through 'signed' and 'unsigned',
+(* CompCert integers' signedness is only interpreted through 'signed' and 'unsigned',
    and not in the representation. Therefore, uints are just names for their respective ints.
-   *)
+ *)
 
-  Notation declassify_usize_from_uint8 := (lift1_both declassify_usize_from_uint8).
-  Notation declassify_u32_from_uint32 := (lift1_both declassify_u32_from_uint32).
+Notation declassify_usize_from_uint8 := (lift1_both declassify_usize_from_uint8).
+Notation declassify_u32_from_uint32 := (lift1_both declassify_u32_from_uint32).
 
-  Notation uint8_rotate_left := (lift2_both uint8_rotate_left).
+Notation uint8_rotate_left := (lift2_both uint8_rotate_left).
 
-  Notation uint8_rotate_right := (lift2_both uint8_rotate_right).
+Notation uint8_rotate_right := (lift2_both uint8_rotate_right).
 
-  Notation uint16_rotate_left := (lift2_both uint16_rotate_left).
+Notation uint16_rotate_left := (lift2_both uint16_rotate_left).
 
-  Notation uint16_rotate_right := (lift2_both uint16_rotate_right).
+Notation uint16_rotate_right := (lift2_both uint16_rotate_right).
 
-  Notation uint32_rotate_left := (lift2_both uint32_rotate_left).
+Notation uint32_rotate_left := (lift2_both uint32_rotate_left).
 
-  Notation uint32_rotate_right := (lift2_both uint32_rotate_right).
+Notation uint32_rotate_right := (lift2_both uint32_rotate_right).
 
-  Notation uint64_rotate_left := (lift2_both uint64_rotate_left).
+Notation uint64_rotate_left := (lift2_both uint64_rotate_left).
 
-  Notation uint64_rotate_right := (lift2_both uint64_rotate_right).
+Notation uint64_rotate_right := (lift2_both uint64_rotate_right).
 
-  Notation uint128_rotate_left := (lift2_both uint128_rotate_left).
+Notation uint128_rotate_left := (lift2_both uint128_rotate_left).
 
-  Notation uint128_rotate_right := (lift2_both uint128_rotate_right).
-  Notation usize_shift_right_ := (lift2_both (fun u s => u usize_shift_right s)).
+Notation uint128_rotate_right := (lift2_both uint128_rotate_right).
+Notation usize_shift_right_ := (lift2_both (fun u s => u usize_shift_right s)).
 
-  Notation usize_shift_left_ :=
-    (fun (u: both (fset []) ([interface]) uint_size) (s: both (fset []) ([interface]) int32) =>
-    {|
-      is_pure := (is_pure u) usize_shift_left (is_pure s) ;
-      is_state :=
-      {code
-         temp_u ← is_state u ;;
-         temp_s ← is_state s ;;
-         ret (temp_u usize_shift_left temp_s)
-      }
-    |}).
-  (* Next Obligation. *)
-  (*   intros. *)
-  (*   pattern_both Hb Hf Hg. *)
-  (*   apply (@r_bind_trans_both (uint_size) (uint_size)). *)
-  (*   subst Hf Hg Hb ; hnf. *)
-  (*   pattern_both Hb Hf Hg. *)
-  (*   apply (@r_bind_trans_both (int32)). *)
-  (*   subst Hf Hg Hb ; hnf. *)
-  (*   apply r_ret. *)
-  (*   easy. *)
-  (* Qed. *)
+Notation usize_shift_left_ :=
+  (fun (u: both (fset []) ([interface]) uint_size) (s: both (fset []) ([interface]) int32) =>
+     {|
+       is_pure := (is_pure u) usize_shift_left (is_pure s) ;
+       is_state :=
+         {code
+            temp_u ← is_state u ;;
+          temp_s ← is_state s ;;
+          ret (temp_u usize_shift_left temp_s)
+         }
+     |}).
+(* Next Obligation. *)
+(*   intros. *)
+(*   pattern_both Hb Hf Hg. *)
+(*   apply (@r_bind_trans_both (uint_size) (uint_size)). *)
+(*   subst Hf Hg Hb ; hnf. *)
+(*   pattern_both Hb Hf Hg. *)
+(*   apply (@r_bind_trans_both (int32)). *)
+(*   subst Hf Hg Hb ; hnf. *)
+(*   apply r_ret. *)
+(*   easy. *)
+(* Qed. *)
 
-  (**** Operations *)
+(**** Operations *)
 
-  Notation shift_left_ := (lift2_both shift_left_).
-  Notation shift_right_ := (lift2_both shift_right_).
+Notation shift_left_ := (lift2_both shift_left_).
+Notation shift_right_ := (lift2_both shift_right_).
 
 (* End Uint. *)
 
@@ -217,3 +219,35 @@ Infix "usize_shift_left" := (usize_shift_left_) (at level 77) : hacspec_scope.
 
 Infix "shift_left" := (shift_left_) (at level 77) : hacspec_scope.
 Infix "shift_right" := (shift_right_) (at level 77) : hacspec_scope.
+
+Program Instance int_add_inst {ws : wsize} : t_Add (@int ws) (@int ws) := {
+    f_Output := int ws ;
+    f_add_loc := fset [] ;
+    f_add {L1 L2 I1 I2} a b := int_add a b
+  }.
+Solve All Obligations with now intros ; rewrite <- fset0E, fsetU0.
+Fail Next Obligation.
+
+Program Instance int_sub_inst {ws : wsize} : t_Sub (@int ws) (@int ws) := {
+    f_Output := int ws ;
+    f_sub_loc := fset [] ;
+    f_sub {L1 L2 I1 I2} a b := int_sub a b
+  }.
+Solve All Obligations with now intros ; rewrite <- fset0E, fsetU0.
+Fail Next Obligation.
+
+Program Instance int_mul_inst {ws : wsize} : t_Mul (@int ws) (@int ws) := {
+    f_Output := int ws ;
+    f_mul_loc := fset [] ;
+    f_mul {L1 L2 I1 I2} a b := int_mul a b
+  }.
+Solve All Obligations with now intros ; rewrite <- fset0E, fsetU0.
+Fail Next Obligation.
+
+Program Instance int_xor_inst {ws : wsize} : t_Xor (@int ws) (@int ws) := {
+    f_Output := int ws ;
+    f_xor_loc := fset [] ;
+    f_xor {L1 L2 I1 I2} a b := int_xor a b
+  }.
+Solve All Obligations with now intros ; rewrite <- fset0E, fsetU0.
+Fail Next Obligation.
