proof-libs/coq/ssprove/src/Hacspec_Lib_Loops.v
@@ -58,10 +58,10 @@ Section Loops.
     | 0 => lift_both cur
     | S n' => foldi_ n' (int_add i (ret_both one)) f (f i cur)
     end.
-  Solve All Obligations with (intros ; (fset_equality || solve_in_fset)).
+  Solve All Obligations with (intros ; solve [fset_equality | solve_in_fset]).
   Fail Next Obligation.
 
-  (* Obligation Tactic := (intros ; (fset_equality || solve_in_fset)). *)
+  (* Obligation Tactic := (intros ; solve [fset_equality | solve_in_fset]). *)
   Equations foldi_both_
            {acc : choice_type}
            (fuel : nat)
@@ -77,7 +77,7 @@ Section Loops.
       | 0 => lift_both cur
       | S n' => solve_lift foldi_both_ n' (int_add i (ret_both one)) (fun x y => solve_lift f (solve_lift x) y) (f i (solve_lift cur))
       end.
-  Solve All Obligations with (intros ; (fset_equality || solve_in_fset)).
+  Solve All Obligations with (intros ; solve [fset_equality | solve_in_fset]).
   Fail Next Obligation.
 
   Equations foldi
@@ -100,7 +100,7 @@ Section Loops.
       | Zpos p => foldi_both_ (Pos.to_nat p) (solve_lift (ret_both lo)) (@f) init (* (fsubset_loc1 := fsubset_loc1) (fsubset_opsig1 := fsubset_opsig1) *)
       end))
   .
-  Solve All Obligations with (intros ; (fset_equality || solve_in_fset)).
+  Solve All Obligations with (intros ; solve [fset_equality | solve_in_fset]).
   Fail Next Obligation.
 
   (* Fold done using natural numbers for bounds *)
